Added some proofs.

Network-Layer/theories/networklayer.v
@@ -1,62 +1,181 @@
 From Coq Require Import Bool.Bool.
 From Coq Require Import Init.Nat.
 From Coq Require Import Lists.List.
+Require Import Omega.
 
-Record regMem := mkMem 
+Record regMem (X : Type) := mkMem 
 {
     address : nat;
-    key : nat
+    key : nat;
+    value : X
 }.
 
-Definition isDesc (a k: nat) (r : regMem) : bool := 
+Definition isDesc {X: Type} (a k: nat) (r : regMem X): bool := 
 match r with
 | {| address := a'; key := k'|} => (eqb a' a) && (eqb k' k)
 end.
 
-Definition getAddr (r : regMem) : nat := 
+Definition getAddr {X: Type} (r : regMem X) : nat := 
 match r with
 | {| address := a'; key := _|} => a'
 end.
 
-Definition getKey (r : regMem) : nat := 
+Definition getKey {X: Type} (r : regMem X) : nat := 
 match r with
 | {| address := _; key := k'|} => k'
 end.
 
+Definition getValue {X: Type} (r : regMem X) : X := 
+match r with
+| {| value := v|} => v
+end.
 
-Record node := mkNode 
+Definition setValue {X : Type} (v : X) (r : regMem X) : regMem X :=
+match r with
+| {| address := a; key := k; value := v'|} => mkMem X a k v
+end.
+
+Record node (X : Type) := mkNode 
 {
     crashed : bool;
-    regions : list regMem;
-    regionUnique : forall (r r' : regMem) regions, 
+    regions : list (regMem X);
+    regionUnique : forall (r r' : regMem X) regions, 
         In r regions /\ In r' regions -> (getAddr r = getAddr r' <-> getKey r = getKey r')
 }.
 
-Fixpoint inRegMem (a k : nat) (l : list regMem) : bool :=
+Fixpoint inRegMem {X: Type} (a k : nat) (l : list (regMem X)) : option X :=
 match l with
 | cons x l' => match isDesc a k x with
-               | true => true
+               | true => Some (getValue x)
                | false => inRegMem a k l'
                end
-| nil => false
+| nil => None
 end.
 
-Definition read (address key : nat) (node : node) 
-: bool := 
-match node with
-| {| regions := l; crashed := c |} => (inRegMem address key l) && negb c
+Fixpoint setRegMem {X: Type} (a k : nat) (v : X) (prev : list (regMem X)) (l : list (regMem X)) : prod (bool) (list (regMem X)) :=
+match l with
+| cons x l' => match isDesc a k x with
+               | true => pair true (prev ++ (cons (setValue v x) l'))
+               | false => setRegMem a k v (prev ++ cons x nil) l'
+               end
+| nil => pair false prev
 end.
 
-Definition write (address key : nat) (node : node) 
-: bool := 
-match node with
-| {| regions := l; crashed := c |} => (inRegMem address key l) && negb c
+Definition frst {X Y : Type} (p : prod X Y) : X := 
+match p with
+| pair x y => x
 end.
 
-Definition isCrashed (node : node)  : bool := 
+Definition scnd {X Y : Type} (p : prod X Y) : Y := 
+match p with
+| pair x y => y
+end.
+
+Definition optionToPair {X : Type} (o : option X) (default : X) : prod bool X :=
+match o with
+| Some x => pair true x
+| None => pair false default
+end.
+
+Lemma someEq : forall (X: Type) (a b : X), Some a = Some b <-> a = b.
+Proof.
+    intros; split; intros.
+    - injection H. auto.
+    - rewrite H. reflexivity.
+Qed.
+
+Lemma someNeq : forall (X: Type) (a b : X), Some a <> Some b <-> a <> b.
+Proof.
+    intros; split; intros; unfold not; intros.
+    - intuition. apply H. rewrite H0. reflexivity.
+    - intuition. apply H. apply -> someEq in H0. apply H0.
+Qed.
+
+Lemma someEq2 : forall (X: Type) (a : X) (o : option X), Some a = o -> (exists b, o = Some b /\ a = b).
+Proof.
+    intros.
+    exists a.
+    rewrite H.
+    auto.
+Qed.
+
+Lemma inRegMemLemma1 : forall (X: Type) (a k: nat) (r : regMem X) (l : list (regMem X)), inRegMem a k (r :: l) = None -> isDesc a k r = false /\ inRegMem a k l = None.
+Proof.
+    intros.
+    split; simpl in H; destruct (isDesc a k r); auto.
+    - discriminate H.
+    - discriminate H.
+Qed.
+
+Lemma applyList : forall (X : Type) (l l' : list X) (x : X),
+l ++ x :: l' = l ++ (cons x nil) ++ l'.
+Proof.
+    intros.
+    induction l.
+    - simpl. reflexivity.
+    - simpl. reflexivity.
+Qed.
+
+Lemma setRegMemLemma : forall (X: Type) (a k: nat) (v : X) (l l' : list (regMem X)),
+setRegMem a k v l' l = pair (frst (setRegMem a k v nil l)) (l' ++ scnd (setRegMem a k v nil l)).
+Proof.
+    intros.
+    generalize l'.
+    induction l.
+    - simpl. intros. rewrite app_nil_r. reflexivity.
+    - simpl. destruct (isDesc a k a0).
+      + simpl. reflexivity.
+      + simpl. intros.
+        assert(setRegMem a k v (a0 :: nil) l = 
+        pair (frst (setRegMem a k v (nil) l))
+        ((cons a0 nil) ++ scnd (setRegMem a k v (nil) l))
+        ). {
+            auto.
+        }
+        rewrite H.
+        simpl.
+        assert(l'0 ++ a0 :: scnd (setRegMem a k v nil l) = 
+        l'0 ++ (a0 :: nil) ++ scnd (setRegMem a k v nil l)).
+        { 
+            apply applyList.
+        }
+        rewrite H0.
+        rewrite app_assoc.
+        apply IHl.
+Qed.
+
+Lemma setGetNexistRegMem : forall (X: Type) (a k: nat) (v : X) (l l' : list (regMem X)), 
+inRegMem a k l = None -> setRegMem a k v nil l = pair false l.
+Proof.
+    intros.
+    induction l.
+    - simpl. reflexivity.
+    - apply inRegMemLemma1 in H. destruct H. simpl. rewrite H.
+      apply IHl in H0. rewrite setRegMemLemma. rewrite H0. simpl. reflexivity.
+Qed.
+
+Definition qualifiedOption {X: Type} (o : option X) (b: bool) : option X :=
+match b with 
+| true => o
+| false => None
+end.
+
+Definition read {X: Type} (address key : nat) (n : node X) 
+: prod (option X) (node X) := 
+match n with
+| {| regions := l; crashed := c |} => pair (qualifiedOption (inRegMem address key l) (negb c)) n
+end.
+
+Definition write {X: Type} (address key : nat) (n : node X) 
+: option X := 
+match n with
+| {| regions := l; crashed := c |} => qualifiedOption (inRegMem address key l) (negb c)
+end.
+
+Definition isCrashed {X: Type} (node : node X)  : bool := 
 match node with
 | {|crashed := c|} => c
 end.
 
-Definition send (node : node)  : bool := negb (isCrashed node).
-Definition recv (node : node) : bool := negb (isCrashed node).
+Definition send {X: Type} (node : node X)  : bool := negb (isCrashed node).
+Definition recv {X: Type} (node : node X) : bool := negb (isCrashed node).
